Switch to partial initial states
Intial states are now gmaps/dmaps instead of functions.
Also change operational models to use maps instead of functions for their
states

ArchSemArm/ArmSeqModel.v
@@ -56,93 +56,86 @@ Context (regs_whitelist : option (gset reg)).
 (** A sequential state for bookkeeping reads and writes to registers/memory in
     gmaps, as well as, the initial state *)
 Record seq_state := {
-  initSt : MState.init 1;
-  mem : gmap address (bv 8);
-  regs : gmap reg (bv 64);
+  (** The sequential model is simple enough to use directly a [MState.t] as an
+      internal mutable state *)
+  sst : MState.init 1;
+  (** [written] records addresses that were written to since the start *)
+  written : gset address;
 }.
 
-Global Instance eta_seq_state : Settable seq_state :=
-  settable! Build_seq_state <initSt;mem;regs>.
+Instance eta_seq_state : Settable seq_state :=
+  settable! Build_seq_state <sst;written>.
 
 Notation seqmon := (Exec.t seq_state string).
 
-Definition read_reg_seq_state (reg : reg) (seqst : seq_state) : reg_type reg:=
-  if (seqst.(regs) !! reg) is Some v
-  then regt_of_bv64 v
-  else (seqst.(initSt).(MState.regs) !!! 0%fin) reg.
+Definition read_reg_seq_state (reg : reg) (seqst : seq_state) :
+    option (reg_type reg) :=
+  seqst.(sst).(MState.regs) !!! 0%fin |> dmap_lookup reg.
 
-Definition read_byte_seq_state_flag (seqst : seq_state) (addr : address) :
-    bv 8 * bool :=
-  if (seqst.(mem) !! addr) is Some v
-  then (v, true)
-  else (seqst.(initSt).(MState.memory) addr, false).
+Definition write_reg_seq_state (reg : reg) (val : reg_type reg) :
+    seq_state → seq_state :=
+  set (lookup_total 0%fin ∘ MState.regs ∘ MState.state ∘ sst)
+    (dmap_insert reg val).
 
-Definition read_byte_seq_state (seqst : seq_state) (addr : address) : bv 8 :=
-  fst (read_byte_seq_state_flag seqst addr).
+Definition read_byte_seq_state (seqst : seq_state) (addr : address) : option (bv 8) :=
+  seqst.(sst).(MState.memory) !! addr.
 
 Definition read_mem_seq_state (n : N) (addr : address) (seqst : seq_state) :
-    bv (8 * n) :=
-  addr_range addr n |$> read_byte_seq_state seqst |> bv_of_bytes (8 * n).
+    option (bv (8 * n)) :=
+  addr_range addr n
+  |$> read_byte_seq_state seqst
+  |> list_of_options
+  |$> bv_of_bytes (8 * n).
 
-Definition read_mem_seq_state_flag (n : N) (addr : address) (seqst : seq_state)
-  : bv (8 * n) * bool :=
-  let bf := addr_range addr n |$> read_byte_seq_state_flag seqst in
-  let '(bytes, flags) := split bf in
-    (bv_of_bytes (8 * n) bytes, existsb id flags).
+(** Check if a region of memory was written to or not *)
+Definition mem_was_written (n : N) (addr : address) (seqst : seq_state) : bool :=
+  bool_decide (∃ a ∈ addr_range addr n, a ∈ seqst.(written)).
+
+Definition check_address_space (pas : addr_space) : seqmon unit :=
+  init_pas ← mget (MState.address_space ∘ sst);
+  guard_or "Wrong address space" (pas = init_pas);;
+  mret ().
 
 Fixpoint write_mem_seq_state (addr : address) (bytes : list (bv 8)) : seqmon unit :=
   if bytes is byte :: bytes
   then
-    msetv (lookup addr ∘ mem) (Some byte);;
+    opt ← mget $ read_mem_seq_state (N.of_nat (length bytes)) addr;
+    guard_or "Memory isn't mapped to write" $ is_Some opt;;
+    msetv (lookup addr ∘ MState.memory ∘ MState.state ∘ sst) (Some byte);;
+    mset written (.∪{[addr]});;
     write_mem_seq_state (addr `+Z` 1)%bv bytes
   else mret ().
 
-(** Combines a gmap with a registerMap to a new registerMap that was updated
-    with the values from the gmap *)
-Definition seq_state_to_init_regs (regs_map : gmap reg (bv 64))
-  (regs_vec : vec registerMap 1) : vec registerMap 1 :=
-  [# (λ reg, if (regs_map !! reg) is Some v then regt_of_bv64 v else (regs_vec !!! 0%fin) reg)].
-
-(** Combines a gmap with a memoryMap to a new memoryMap that was updated with the
-    values from the gmap *)
-Definition seq_state_to_init_mem (mem_map : gmap address (bv 8)) (mem : memoryMap)
-  : memoryMap :=
-  λ addr, if (mem_map !! addr) is Some v then v else mem addr.
-
-(** Turn a seq_state into an MState.init by updating the initial state with the
-    gmaps for registers and memory *)
-Definition seq_state_to_init (seqs : seq_state) : MState.init 1 :=
-  {| MState.state :=
-      {| MState.memory :=
-          seq_state_to_init_mem seqs.(mem) seqs.(initSt).(MState.memory);
-         MState.address_space := ();
-         MState.regs :=
-          seq_state_to_init_regs seqs.(regs) seqs.(initSt).(MState.regs) |};
-     MState.termCond := seqs.(initSt).(MState.termCond) |}.
-
 (** This is the effect handler for the outcome effect in the sequential model *)
 Equations sequential_model_outcome (call : outcome) : seqmon (eff_ret call) :=
-  | RegRead reg racc => mget (read_reg_seq_state reg)
+  | RegRead reg racc =>
+      opt ←  mget (read_reg_seq_state reg);
+      Exec.error_none "Register not found" opt
   | RegWrite reg racc val =>
-    if regs_whitelist is Some rwl
-    then if bool_decide (reg ∈ rwl)
-      then msetv (lookup reg ∘ regs) (Some (regt_to_bv64 val))
-      else mthrow "Write to illegal register"
-    else msetv (lookup reg ∘ regs) (Some (regt_to_bv64 val))
+      opt ←  mget (read_reg_seq_state reg);
+      guard_or "Writing register not in initial state" $ is_Some opt;;
+      if regs_whitelist is Some rwl
+      then
+        if bool_decide (reg ∈ rwl)
+        then mSet $ write_reg_seq_state reg val
+        else mthrow "Write to illegal register (not in whitelist)"
+      else mSet $ write_reg_seq_state reg val
   | MemRead n 0 rr =>
-    if is_ifetch rr.(ReadReq.access_kind) || is_ttw rr.(ReadReq.access_kind)
-    then
-      '(read, flag) ← mget (read_mem_seq_state_flag n rr.(ReadReq.address));
-      if (flag : bool)
-      then mthrow "iFetch or TTW read from modified memory"
-      else mret (Ok (read, bv_0 _))
-    else
-      read ← mget (read_mem_seq_state n rr.(ReadReq.address));
+      check_address_space rr.(ReadReq.address_space);;
+      ( if is_ifetch rr.(ReadReq.access_kind) || is_ttw rr.(ReadReq.access_kind)
+        then
+          was_written ← mget (mem_was_written n rr.(ReadReq.address));
+          guard_or "Ifetch or TTW reading from modified memory" (negb was_written);;
+          mret ()
+        else mret ());;
+      opt ← mget (read_mem_seq_state n rr.(ReadReq.address));
+      read ← Exec.error_none "Memory not found" opt;
       mret (Ok (read, bv_0 _))
   | MemRead _ _ _ => mthrow "CHERI tags are unsupported for now"
-  | MemWriteAddrAnnounce _ _ _ _ _ => mret ()
+  | MemWriteAddrAnnounce _ _ _ _ pas => check_address_space pas
   | MemWrite n 0 wr =>
-    write_mem_seq_state wr.(WriteReq.address) (wr.(WriteReq.value) |> bv_to_bytes 8);;
+      check_address_space wr.(WriteReq.address_space);;
+      write_mem_seq_state wr.(WriteReq.address) (wr.(WriteReq.value) |> bv_to_bytes 8);;
     mret (Ok ())
   | MemWrite _ _ _ => mthrow "CHERI tags are unsupported for now"
   | Barrier _ => mret ()
@@ -160,7 +153,7 @@ Fixpoint sequential_model_seqmon (fuel : nat) (isem : iMon ())
   if fuel is S fuel
   then
     FMon.cinterp sequential_model_outcome isem;;
-    st ← mget seq_state_to_init;
+    st ← mget sst;
     if MState.finalize st is Some final
     then mret final
     else sequential_model_seqmon fuel isem
@@ -173,7 +166,7 @@ Definition sequential_modelc (fuel : nat) (isem : iMon ()) : (Model.c ∅) :=
   λ n,
   match n with
   | 1 => λ initSt : MState.init 1,
-    {| initSt := initSt; regs := ∅; mem := ∅ |}
+    {| sst := initSt; written := ∅ |}
     |> Model.Res.from_exec (sequential_model_seqmon fuel isem)
   | _ => λ _, mret (Model.Res.Error "Exptected one thread")
   end.
