ArchSemArm/VMPromising.v
@@ -52,6 +52,7 @@ Require Import ASCommon.HVec.
 Require Import Coq.Program.Equality.
 
 Require UMPromising.
+Import (hints) UMPromising.
 
 Require Import ArchSem.GenPromising.
 Require Import ArmInst.
@@ -62,7 +63,6 @@ From stdpp Require Import pretty.
 
 (* Shadow constructor name from coq-sail with our result type *)
 Import ASCommon.CResult.
-
 
 #[local] Open Scope stdpp.
 
@@ -177,11 +177,21 @@ Module Memory.
   (** Representation of initial memory, this is representation
       optimized for the internals of this model, so it not a plain
       memoryMap *)
-  Definition initial := Loc.t -> val.
+  Definition initial := gmap Loc.t val.
+  #[export] Typeclasses Transparent initial.
 
   (** Convert from a memoryMap to the internal representation: initial *)
   Definition initial_from_memMap (mem : memoryMap) : initial :=
-    fun loc => Loc.to_addrs loc |> map mem |> bv_of_bytes 64.
+    mem
+    |> dom
+    |> (set_map (bv_extract 3 53) : _ → gset Loc.t)
+    |> set_fold (λ loc map,
+          let val :=
+            for addr in addr_range (Loc.to_addr loc) 8 do mem !! addr end
+            |$> bv_of_bytes 64
+          in
+          partial_alter (λ _, val) loc map) ∅.
+
 
   (** The promising memory: a list of events *)
   Definition t : Type := t Ev.t.
@@ -195,15 +205,16 @@ Module Memory.
  (** Reads the last write to a location in some memory. Gives the value and the
      timestamp of the write that it read from.
      The timestamp is 0 if reading from initial memory. *)
-  Fixpoint read_last (loc : Loc.t) (init : initial) (mem : t) : (val * nat) :=
+  Fixpoint read_last (loc : Loc.t) (init : initial) (mem : t) : option (val * nat) :=
     match mem with
-    | [] => (init loc, 0%nat)
+    | [] => init !! loc |$> (., 0%nat)
     | (Ev.Msg msg) :: mem' =>
         if Msg.loc msg =? loc then
-          (Msg.val msg, List.length mem)
+          Some (Msg.val msg, List.length mem)
         else read_last loc init mem'
     | Ev.Tlbi _ :: mem' => read_last loc init mem'
     end.
+
 
   (** Read memory at a given timestamp without any weak memory behaviour *)
   Definition read_at (loc : Loc.t) (init : initial) (mem : t) (time : nat) :=
@@ -214,9 +225,10 @@ Module Memory.
       This is mainly for instruction fetching in this model *)
   Definition read_initial (loc : Loc.t) (init : initial) (mem : t) : option val :=
     match read_last loc init mem with
-    | (v, 0%nat) => Some v
+    | Some (v, 0%nat) => Some v
     | _ => None
     end.
+
 
   (* (** Reads from initial memory for instruction fetch (only 4 bytes aligned) *)
   (*     and fail if the memory was modified *)
@@ -235,47 +247,38 @@ Module Memory.
   (*   end. *)
 
 
-
   (** Transform a promising initial memory and memory history back to a
       TermModel memoryMap *)
-  Definition to_memMap (init : initial) (mem : t) : memoryMap :=
-    fun addr =>
-      let loc := Loc.from_addr_in addr in
-      let '(v, _) := read_last loc init mem in
-      let index := Loc.addr_index addr in
-      bv_to_bytes 8 v !! bv_unsigned index |> default (bv_0 8).
-
-  (** Adds the view number to each message given a view for the last message.
-      This is for convenient use with cut_after.
-
-      TODO: it would make sense to make a function that does cut_after
-      and this in a single step. *)
-  (* Fixpoint with_views_from (v : view) (mem : t) *)
-  (*   : list (Msg.t * view) := *)
-  (*   match mem with *)
-  (*   | [] => [] *)
-  (*   | h :: q => (v, h) :: with_views_from (v - 1) q *)
-  (*   end. *)
-
+  Definition to_memMap (init : initial) (mem : t) : memoryMap:=
+    let final :=
+      foldl (λ nmem ev,
+          if ev is Ev.Msg msg
+          then insert msg.(Msg.loc) msg.(Msg.val) nmem
+          else nmem)
+        init mem
+    in
+    map_fold (λ loc (val : bv 64), mem_insert (Loc.to_addr loc) 8 val) ∅ final.
 
   (** Returns the list of possible reads at a location restricted by a certain
       view. The list is never empty as one can always read from at least the
       initial value. *)
   Definition read (loc : Loc.t) (v : view) (init : initial) (mem : t)
-    : list (val * view) :=
-    let first := mem |> cut_before v |> read_last loc init in
-    let lasts := mem |> cut_after_with_timestamps v
-                     |> list_filter_map
-                     (fun '(ev, v) =>
-                        match ev with
-                        | Ev.Msg msg =>
-                            if Msg.loc msg =? loc
-                            then Some (Msg.val msg, v)
-                            else None
-                        | Ev.Tlbi _ => None
-                        end)
+    : option (list (val * view)) :=
+    first ← mem |> cut_before v |> read_last loc init;
+    let lasts :=
+      mem |> cut_after_with_timestamps v
+      |> list_filter_map
+           (λ '(ev, v),
+             match ev with
+             | Ev.Msg msg =>
+                 if Msg.loc msg =? loc
+                 then Some (Msg.val msg, v)
+                 else None
+             | Ev.Tlbi _ => None
+             end)
     in
-    lasts ++ [first].
+    Some (lasts ++ [first])%list.
+
 
   (** Promise a write and add it at the end of memory *)
   Definition promise (ev : Ev.t) : Exec.t t string view :=
@@ -337,252 +340,90 @@ Bind Scope fin_scope with ELp.
 Definition ELp_to_EL : ELp -> EL := FS.
 
 
+(** * Register classification
 
-(** Any write to a register not explicitly supported by Reg.t will fail,
-    because this means that the model doesn't know which behavior it is supposed to
-    have *)
-Module Reg.
-  (** application/non-relaxed registers *)
-  Inductive app :=
-  | R (num : fin 31)
-  | SP (el : EL)
-  | ELR (el : ELp)
-  | PSTATE.
+    Here we classify register based on which category they belong to. Register
+    that are not listed here (other than the PC) are unsupported and cannot be
+    written to (But can be read if unmodified) *)
 
-  #[global] Instance app_eq_dec : EqDecision app.
-  Proof. solve_decision. Defined.
+(** Strict registers are those have non-relaxed behaviour: every read must read
+    the previous write e.g GP register, stack pointers, ... *)
+Definition strict_regs : gset reg :=
+  list_to_set [
+      GReg R0;
+      GReg R1;
+      GReg R2;
+      GReg R3;
+      GReg R4;
+      GReg R5;
+      GReg R6;
+      GReg R7;
+      GReg R8;
+      GReg R9;
+      GReg R10;
+      GReg R11;
+      GReg R12;
+      GReg R13;
+      GReg R14;
+      GReg R15;
+      GReg R16;
+      GReg R17;
+      GReg R18;
+      GReg R19;
+      GReg R20;
+      GReg R21;
+      GReg R22;
+      GReg R23;
+      GReg R24;
+      GReg R25;
+      GReg R26;
+      GReg R27;
+      GReg R28;
+      GReg R29;
+      GReg R30;
+      GReg SP_EL0;
+      GReg SP_EL1;
+      GReg SP_EL2;
+      GReg SP_EL3;
+      GReg PSTATE;
+      GReg ELR_EL1;
+      GReg ELR_EL2;
+      GReg ELR_EL3].
 
-  Local Open Scope positive.
+(** Relaxed registers are not guaranteed to read the latest value. *)
+Definition relaxed_regs : gset reg :=
+  list_to_set [
+      GReg ESR_EL1;
+      GReg ESR_EL2;
+      GReg ESR_EL3;
+      GReg FAR_EL1;
+      GReg FAR_EL2;
+      GReg FAR_EL3;
+      GReg PAR_EL1;
+      GReg TTBR0_EL1;
+      GReg TTBR0_EL2;
+      GReg TTBR0_EL3;
+      GReg TTBR1_EL1;
+      GReg TTBR1_EL2;
+      GReg VBAR_EL1;
+      GReg VBAR_EL2;
+      GReg VBAR_EL3;
+      GReg VTTBR_EL2].
 
-  (* TODO Ltac2 tactic to do this *)
-  #[global] Program Instance app_countable : Countable app :=
-    {| encode a :=
-        match a with
-        | R n => (encode n)~0~0
-        | SP el => (encode el)~0~1
-        | ELR el => (encode el)~1~0
-        | PSTATE => 1~0
-        end;
-      decode p :=
-        match p with
-        | n~0~0 => (decode n) |$> R
-        | n~0~1 => (decode n) |$> SP
-        | n~1~0 => (decode n) |$> ELR
-        | 1~0 => Some PSTATE
-        | _ => None
-        end|}.
-  Next Obligation. intros []; by try rewrite decode_encode. Qed.
-
-  (** Relaxed system registers *)
-  Inductive sys :=
-  | ESR (el : ELp)
-  | FAR (el : ELp)
-  | PAR (* EL1 *)
-  | TTBR0 (el : ELp)
-  | TTBR1 (el2 : bool)
-  | VBAR (el : ELp)
-  | VTTBR (* EL2 *).
-
-  #[global] Instance sys_dec : EqDecision sys.
-  solve_decision.
-  Defined.
-
-  #[global] Program Instance sys_countable : Countable sys :=
-    {| encode a :=
-        match a with
-        | ESR el => (encode el)~0~0~0
-        | FAR el => (encode el)~0~0~1
-        | PAR => 1~0
-        | TTBR0 el => (encode el)~0~1~1
-        | TTBR1 el => (encode el)~1~0~0
-        | VBAR el => (encode el)~1~0~1
-        | VTTBR => 1~1~0
-        end;
-      decode p :=
-        match p with
-        | n~0~0~0 => (decode n) |$> ESR
-        | n~0~0~1 => (decode n) |$> FAR
-        | 1~0 => Some PAR
-        | n~0~1~1 => (decode n) |$> TTBR0
-        | n~1~0~0 => (decode n) |$> TTBR1
-        | n~1~0~1 => (decode n) |$> VBAR
-        | 1~1~0 => Some VTTBR
-        | _ => None
-        end|}.
-  Next Obligation. intros []; by try rewrite decode_encode. Qed.
-
-  Inductive t :=
-  | PC
-  | App (app : app)
-  | Sys (sys : sys).
-
-  #[global] Instance eq_dec : EqDecision t.
-  Proof. solve_decision. Defined.
-
-  #[global] Program Instance countable : Countable t :=
-    {| encode a :=
-        match a with
-        | PC => 1
-        | App a => (encode a)~0
-        | Sys s => (encode s)~1
-        end;
-      decode p :=
-        match p with
-        | n~0 => (decode n) |$> App
-        | n~1 => (decode n) |$> Sys
-        | 1 => Some PC
-        end|}.
-  Next Obligation. intros []; by try rewrite decode_encode. Qed.
-
-  (* for i in range (0, 31):
-         print(f"    | R{i} => Some (App (R {i}))")*)
-  Definition from_arch (r : reg) : option t :=
-    match r with
-    | _PC => Some PC
-    | R0 => Some (App (R 0))
-    | R1 => Some (App (R 1))
-    | R2 => Some (App (R 2))
-    | R3 => Some (App (R 3))
-    | R4 => Some (App (R 4))
-    | R5 => Some (App (R 5))
-    | R6 => Some (App (R 6))
-    | R7 => Some (App (R 7))
-    | R8 => Some (App (R 8))
-    | R9 => Some (App (R 9))
-    | R10 => Some (App (R 10))
-    | R11 => Some (App (R 11))
-    | R12 => Some (App (R 12))
-    | R13 => Some (App (R 13))
-    | R14 => Some (App (R 14))
-    | R15 => Some (App (R 15))
-    | R16 => Some (App (R 16))
-    | R17 => Some (App (R 17))
-    | R18 => Some (App (R 18))
-    | R19 => Some (App (R 19))
-    | R20 => Some (App (R 20))
-    | R21 => Some (App (R 21))
-    | R22 => Some (App (R 22))
-    | R23 => Some (App (R 23))
-    | R24 => Some (App (R 24))
-    | R25 => Some (App (R 25))
-    | R26 => Some (App (R 26))
-    | R27 => Some (App (R 27))
-    | R28 => Some (App (R 28))
-    | R29 => Some (App (R 29))
-    | R30 => Some (App (R 30))
-    | SP_EL0 => Some (App (SP 0))
-    | SP_EL1 => Some (App (SP 1))
-    | SP_EL2 => Some (App (SP 2))
-    | SP_EL3 => Some (App (SP 3))
-    | System_types.PSTATE => Some (App PSTATE)
-    | ELR_EL1 => Some (App (ELR 0))
-    | ELR_EL2 => Some (App (ELR 1))
-    | ELR_EL3 => Some (App (ELR 2))
-    | ESR_EL1 => Some (Sys (ESR 0))
-    | ESR_EL2 => Some (Sys (ESR 1))
-    | ESR_EL3 => Some (Sys (ESR 2))
-    | FAR_EL1 => Some (Sys (FAR 0))
-    | FAR_EL2 => Some (Sys (FAR 1))
-    | FAR_EL3 => Some (Sys (FAR 2))
-    | PAR_EL1 => Some (Sys PAR)
-    | TTBR0_EL1 => Some (Sys (TTBR0 0))
-    | TTBR0_EL2 => Some (Sys (TTBR0 1))
-    | TTBR0_EL3 => Some (Sys (TTBR0 2))
-    | TTBR1_EL1 => Some (Sys (TTBR1 false))
-    | TTBR1_EL2 => Some (Sys (TTBR1 true))
-    | VBAR_EL1 => Some (Sys (VBAR 0))
-    | VBAR_EL2 => Some (Sys (VBAR 1))
-    | VBAR_EL3 => Some (Sys (VBAR 2))
-    | VTTBR_EL2 => Some (Sys VTTBR)
-    end.
-
-
-  Equations to_arch : t → Arm.Arch.reg :=
-  | PC => _PC;
-  | App (R 0) => R0;
-  | App (R 1) => R1;
-  | App (R 2) => R2;
-  | App (R 3) => R3;
-  | App (R 4) => R4;
-  | App (R 5) => R5;
-  | App (R 6) => R6;
-  | App (R 7) => R7;
-  | App (R 8) => R8;
-  | App (R 9) => R9;
-  | App (R 10) => R10;
-  | App (R 11) => R11;
-  | App (R 12) => R12;
-  | App (R 13) => R13;
-  | App (R 14) => R14;
-  | App (R 15) => R15;
-  | App (R 16) => R16;
-  | App (R 17) => R17;
-  | App (R 18) => R18;
-  | App (R 19) => R19;
-  | App (R 20) => R20;
-  | App (R 21) => R21;
-  | App (R 22) => R22;
-  | App (R 23) => R23;
-  | App (R 24) => R24;
-  | App (R 25) => R25;
-  | App (R 26) => R26;
-  | App (R 27) => R27;
-  | App (R 28) => R28;
-  | App (R 29) => R29;
-  | App (R 30) => R30;
-  | App (SP 0) => SP_EL0;
-  | App (SP 1) => SP_EL1;
-  | App (SP 2) => SP_EL2;
-  | App (SP 3) => SP_EL3;
-  | App PSTATE => System_types.PSTATE;
-  | App (ELR 0) => ELR_EL1;
-  | App (ELR 1) => ELR_EL2;
-  | App (ELR 2) => ELR_EL3;
-  | Sys (ESR 0) => ESR_EL1;
-  | Sys (ESR 1) => ESR_EL2;
-  | Sys (ESR 2) => ESR_EL3;
-  | Sys (FAR 0) => FAR_EL1;
-  | Sys (FAR 1) => FAR_EL2;
-  | Sys (FAR 2) => FAR_EL3;
-  | Sys PAR => PAR_EL1;
-  | Sys (TTBR0 0) => TTBR0_EL1;
-  | Sys (TTBR0 1) => TTBR0_EL2;
-  | Sys (TTBR0 2) => TTBR0_EL3;
-  | Sys (TTBR1 false) => TTBR1_EL1;
-  | Sys (TTBR1 true) => TTBR1_EL2;
-  | Sys (VBAR 0) => VBAR_EL1;
-  | Sys (VBAR 1) => VBAR_EL2;
-  | Sys (VBAR 2) => VBAR_EL3;
-  | Sys VTTBR => VTTBR_EL2.
-
-
-  Ltac fin_case :=
-    match goal with
-    | n : fin 0 |- _ => dep_destruct n
-    | n : fin _ |- _ => dep_destruct n; [| clear n]
-    end.
-
-  Lemma to_from_arch (reg : t) : from_arch (to_arch reg) = Some reg.
-  Proof. funelim (to_arch reg); cbn; reflexivity. Qed.
-
-  Lemma from_to_arch (r : reg) (r' : t) : (from_arch r) = Some r' -> to_arch r' = r.
-  Proof. destruct r as [_ [[]]]; cdestruct r' |- ***.
-  Qed.
-
-End Reg.
-Coercion Reg.App : Reg.app >-> Reg.t.
-Coercion Reg.Sys : Reg.sys >-> Reg.t.
+(** * The thread state *)
 
 Module WSReg.
   Record t :=
     make {
-        sreg : Reg.sys;
-        val : bv 64;
+        sreg : reg;
+        val : reg_type sreg;
         view : nat
       }.
 
-
-  Definition to_val_view (wsreg : t) := (wsreg.(val), wsreg.(view)).
+  Definition to_val_view_if (sr : reg) (wsreg : t) : option (reg_type sr * nat) :=
+    if decide (wsreg.(sreg) = sr) is left eq
+    then Some $ (ctrans eq wsreg.(val), wsreg.(view))
+    else None.
 End WSReg.
 
 
@@ -595,15 +436,14 @@ Module TState.
            Is must be ordered with oldest promises at the bottom of the list *)
         prom : list view;
 
-        (* registers values and views *)
-        pc : bv 64;
-        regs : Reg.app -> bv 64 * view;
-        regs_init : registerMap;
+        (* registers values and views. System(relaxed) registers are not
+           modified in the [regs] field directly, but instead accumulate changes *)
+        regs : dmap reg (λ reg, reg_type reg * view)%type;
         (* TODO: levents *)
         sregs : list WSReg.t;
 
         (* The coherence views *)
-        coh : Loc.t -> view;
+        coh : gmap Loc.t view;
 
         vrd : view; (* The maximum output view of a read  *)
         vwr : view; (* The maximum output view of a write  *)
@@ -620,7 +460,7 @@ Module TState.
         (* Forwarding database. The first view is the timestamp of the
            write while the second view is the max view of the dependencies
            of the write. The boolean marks if the store was an exclusive*)
-        fwdb : Loc.t -> FwdItem.t;
+        fwdb : gmap Loc.t FwdItem.t;
 
         (* Exclusive database. If there was a recent load exclusive but the
            corresponding store exclusive has not yet run, this will contain
@@ -638,18 +478,16 @@ Module TState.
       }.
 
   #[global] Instance eta : Settable _ :=
-    settable! make <prom;pc;regs;regs_init;sregs;coh;vrd;vwr;vdmbst;vdmb;vdsb;
+    settable! make <prom;regs;sregs;coh;vrd;vwr;vdmbst;vdmb;vdsb;
                     vspec;vcse;vtlbi;vmsr;vacq;vrel;fwdb;xclb;scse;tlbscses>.
 
   (* TODO Check and remove mem as an argument here *)
   Definition init (mem : memoryMap) (iregs : registerMap) :=
     ({|
       prom := [];
-      pc := iregs (Reg.to_arch Reg.PC);
-      regs := fun reg => (regt_to_bv64 (iregs (Reg.to_arch reg)), 0);
-      regs_init := iregs;
+      regs := dmap_map (λ _ v, (v, 0%nat)) iregs;
       sregs := []; (* latest event at the top of the list *)
-      coh := fun loc => 0;
+      coh := ∅;
       vrd := 0;
       vwr := 0;
       vdmbst := 0;
@@ -661,7 +499,7 @@ Module TState.
       vmsr := 0;
       vacq := 0;
       vrel := 0;
-      fwdb := fun loc => FwdItem.init;
+      fwdb := ∅;
       xclb := None;
       scse := 0;
       tlbscses := (fun _ => None)
@@ -670,83 +508,81 @@ Module TState.
   Definition sreg_cur (ts : t) := length ts.(sregs).
 
   (** Read the last system register write at system register position s *)
-  Definition read_sreg_last (ts : t) (s : nat) (sreg : Reg.sys) :=
-    ts.(sregs)
-         |> drop ((sreg_cur ts) - s)
-         |> filter (fun wsreg => wsreg.(WSReg.sreg) = sreg)
-         |> hd_error
-         |> fmap (M:= option) WSReg.to_val_view
-         |> default (ts.(regs_init) (Reg.to_arch sreg)|> regt_to_bv64, 0%nat).
+  Definition read_sreg_last (ts : t) (s : nat) (sreg : reg) :=
+    let newval :=
+      ts.(sregs)
+      |> drop ((sreg_cur ts) - s)
+      |> list_filter_map (WSReg.to_val_view_if sreg)
+      |> hd_error in
+    newval ∪ dmap_lookup sreg ts.(regs).
 
   (** Read all possible system register values for sreg assuming the last
       synchronization at position sync *)
-  Definition read_sreg (ts : t) (sync : nat) (sreg : Reg.sys)
-    : list (bv 64 * view)
+  Definition read_sreg (ts : t) (sync : nat) (sreg : reg)
+    : option (list (reg_type sreg * view))
     :=
+    sync_val ← read_sreg_last ts sync sreg;
     let rest :=
       ts.(sregs)
-           |> take ((sreg_cur ts) - sync)
-           |> filter (fun wsreg => wsreg.(WSReg.sreg) = sreg)
-           |> map WSReg.to_val_view
-    in (read_sreg_last ts sync sreg) :: rest.
+      |> take ((sreg_cur ts) - sync)
+      |> list_filter_map (WSReg.to_val_view_if sreg)
+    in Some $ sync_val :: rest.
 
   (** Read uniformly a register of any kind. *)
-  Definition read_reg (ts : t) (r : reg) : bv 64 * view :=
-    match Reg.from_arch r with
-    | Some Reg.PC => (ts.(pc),0%nat)
-    | Some (Reg.App app) => ts.(regs) app
-    | Some (Reg.Sys sys) => read_sreg_last ts (sreg_cur ts) sys
-    | None => (ts.(regs_init) r |> regt_to_bv64, 0%nat)
-    end.
-
+  Definition read_reg (ts : t) (r : reg) : option (reg_type r * view) :=
+    if bool_decide (r ∈ relaxed_regs) then
+      read_sreg_last ts (sreg_cur ts) r
+    else dmap_lookup r ts.(regs).
 
   (** Extract a plain register map from the thread state without views.
       This is used to decide if a thread has terminated, and to observe the
       results of the model *)
   Definition reg_map (ts : t) : registerMap :=
-    λ r, regt_of_bv64 (read_reg ts r).1.
+    dmap_map (λ _, fst) ts.(regs).
 
   (** Sets the value of a register *)
-  Definition set_reg (reg : Reg.app) (rv : bv 64 * view) : t -> t
-    := set regs (fun_add reg rv).
+  Definition set_reg (reg : reg) (rv : reg_type reg * view) (ts : t) : option t :=
+    if decide (is_Some (dmap_lookup reg ts.(regs))) then
+      Some $ set regs (dmap_insert reg rv) ts
+    else None.
 
   (** Sets the coherence view of a location *)
-  Definition set_coh (loc : Loc.t) (v : view) : t -> t :=
-    set coh (fun_add loc v).
+  Definition set_coh (loc : Loc.t) (v : view) : t → t :=
+    set coh (insert loc v).
 
   (** Updates the coherence view of a location by taking the max of the new
       view and of the existing value *)
-  Definition update_coh (loc : Loc.t) (v : view) (s : t) : t :=
-    set_coh loc (max v (coh s loc)) s.
+  Definition update_coh (loc : Loc.t) (v : view) : t → t :=
+    set coh (alter (max v) loc).
 
   (** Updates the forwarding database for a location. *)
-  Definition set_fwdb (loc : Loc.t) (fi : FwdItem.t) : t -> t :=
-    set fwdb (fun_add loc fi).
+  Definition set_fwdb (loc : Loc.t) (fi : FwdItem.t) : t → t :=
+    set fwdb (insert loc fi).
 
   (** Set the exclusive database to the timestamp and view of the latest
       load exclusive *)
-  Definition set_xclb (vs : view * view) : t -> t :=
-    set xclb (fun _ => Some vs).
+  Definition set_xclb (vs : view * view) : t → t :=
+    set xclb (λ _, Some vs).
 
   (** Clear the exclusive database, to mark a store exclusive *)
-  Definition clear_xclb : t -> t :=
-    set xclb (fun _ => None).
+  Definition clear_xclb : t → t :=
+    set xclb (λ _, None).
 
   (** Updates a view that from the state, by taking the max of new value and
       the current value.
 
-      For example `update rmax vnew t` does t.rmax <- max t.rmax vnew *)
-  Definition update (acc : t -> view) {_: Setter acc}
-             (v : view) : t -> t :=
+      For example `update rmax vnew t` does t.rmax ← max t.rmax vnew *)
+  Definition update (acc : t → view) {_: Setter acc}
+             (v : view) : t → t :=
     set acc (max v).
 
   (** Updates two view in the same way as update. Purely for convenience *)
-  Definition update2 (acc1 acc2 : t -> view) {_: Setter acc1} {_: Setter acc2}
-             (v : view) : t -> t :=
+  Definition update2 (acc1 acc2 : t → view) {_: Setter acc1} {_: Setter acc2}
+             (v : view) : t → t :=
     (update acc1 v) ∘ (update acc2 v).
 
   (** Add a promise to the promise set *)
-  Definition promise (v : view) : t -> t := set prom (fun p => v :: p).
+  Definition promise (v : view) : t -> t := set prom (v ::.).
 
   (** Perform a context synchronization event *)
   Definition cse (v : view) (ts : t) : t :=
@@ -880,10 +716,9 @@ Module TLB.
 
   Definition init := make 0 VATLB.init.
 
-  Definition read_sreg (tlb : t) (ts : TState.t) (time : nat)
-    (sreg : Reg.sys) :=
+  Definition read_sreg (tlb : t) (ts : TState.t) (time : view) (sreg : reg) :=
     TState.read_sreg ts tlb.(scse) sreg
-    |> filter (fun '(val, v) => v <= time)%nat.
+    |$> filter (λ '(val, v), v <= time)%nat.
 
 
 
@@ -1067,7 +902,6 @@ Definition read_fwd_view (ak : Explicit_access_kind) (f : FwdItem.t) :=
   then f.(FwdItem.time) else f.(FwdItem.view).
 
 
-
 (** Performs a memory read at a location with a view and return possible output
     states with the timestamp and value of the read *)
 Definition read_mem_explicit (loc : Loc.t) (vaddr : view)
@@ -1085,12 +919,15 @@ Definition read_mem_explicit (loc : Loc.t) (vaddr : view)
   let vpre := vaddr ⊔ vbob in
   (* We only read after the coherence point, because without mixed-size, this
      is equivalent to reading at vpre and discarding incoherent options *)
-  let vread := vpre ⊔ (TState.coh ts loc) in
+  let vread := vpre ⊔ (TState.coh ts !!! loc) in
   mem ← mget snd;
-  '(res, time) ← Exec.Results $ Memory.read loc vread init mem;
-  let fwd := TState.fwdb ts loc in
+  reads ← Exec.error_none "Reading from unmapped memory" $
+            Memory.read loc vread init mem;
+  '(res, time) ← mchoosel reads;
   let read_view :=
-    if (fwd.(FwdItem.time) =? time) then read_fwd_view ak fwd else time in
+    if (ts.(TState.fwdb) !! loc) is Some fwd then
+      if (fwd.(FwdItem.time) =? time) then read_fwd_view ak fwd else time
+    else time in
   let vpost := vpre ⊔ read_view in
   guard_discard (vpost <= invalidation_time)%nat;;
   mset fst $ TState.update_coh loc time;;
@@ -1178,7 +1015,7 @@ Definition write_mem (tid : nat) (loc : Loc.t) (viio : view) (acs : Access_stren
     ⊔ ts.(TState.vcse) ⊔ ts.(TState.vacq)
     ⊔ view_if is_release (ts.(TState.vrd) ⊔ ts.(TState.vwr)) in
   let vpre := ts.(TState.vspec) ⊔ vbob ⊔ viio in
-  guard_discard (vpre ⊔ (TState.coh ts loc) < time)%nat;;
+  guard_discard (vpre ⊔ (TState.coh ts !!! loc) < time)%nat;;
   mset (TState.prom ∘ fst) $ delete time;;
   mset fst $ TState.update_coh loc time;;
   mset fst $ TState.update TState.vwr time;;
@@ -1315,15 +1152,19 @@ Section RunOutcome.
         (bool_decide (racc ≠ None));;
       iis ← mget PPState.iis;
       let vreg := IIS.strict iis in
-      match Reg.from_arch reg with
-      | Some Reg.PC =>
-          mset PPState.state $ TState.update TState.vspec vreg;;
-          msetv (TState.pc ∘ PPState.state) (regt_to_bv64 val)
-      | Some (Reg.App app) =>
-          mset PPState.state $ TState.set_reg app (regt_to_bv64 val, vreg)
-      | Some (Reg.Sys sys) => mthrow "TODO"
-      | None => mthrow "Writing to unsupported system register"
-      end
+      vreg' ←
+        (if reg =? pc_reg
+         then
+           mset PPState.state $ TState.update TState.vspec vreg;;
+           mret 0%nat
+         else mret vreg);
+      if decide (reg ∈ relaxed_regs) then
+        mthrow "TODO"
+      else
+        ts ← mget PPState.state;
+        nts ← Exec.error_none "Register isn't mapped, can't write" $
+                TState.set_reg reg (val, vreg') ts;
+        msetv PPState.state nts
   | RegRead reg direct => mthrow "TODO"
   | MemRead 8 0 rr =>
       let initmem := Memory.initial_from_memMap initmem in
@@ -1388,9 +1229,6 @@ Definition VMPromising_nocert' : PromisingModel :=
 
 Definition VMPromising_nocert isem :=
   Promising_to_Modelnc isem VMPromising_nocert'.
-
-(* The certified version only works on simple ISA model without internal
-     state *)
 
 Definition seq_step (isem : iMon ()) (tid : nat) (initmem : memoryMap)
   : relation (TState.t * Memory.t) :=
