ArchSemArm/tests/ArmSeqModelTest.v
@@ -12,8 +12,9 @@ Definition r0_extract (a : Model.Res.t ∅ 1) : result string Z :=
   match a with
   | Model.Res.FinalState fs =>
       let regs : registerMap := fs.(MState.regs) !!! 0%fin in
-      let r0 : bv 64 := regs R0 in
-      Ok (bv_unsigned r0)
+      if reg_lookup R0 regs is Some r0
+      then Ok (bv_unsigned r0)
+      else Error "R0 not in state"
   | Model.Res.Error s => Error s
   | Model.Res.Unspecified e => match e with end
   end.
@@ -21,21 +22,20 @@ Definition r0_extract (a : Model.Res.t ∅ 1) : result string Z :=
 
 (* Run EOR X0, X1, X2 at pc address 0x500, whose opcode is 0xca020020 *)
 Module EOR.
-Equations init_reg : registerMap:=
-  init_reg (GReg (R_bitvector_64 _PC)) := 0x500;
-  init_reg (GReg (R_bitvector_64 R0)) := 0x0;
-  init_reg (GReg (R_bitvector_64 R1)) := 0x11;
-  init_reg (GReg (R_bitvector_64 R2)) := 0x101;
-  init_reg _ := 0x0.
 
-Equations init_mem : memoryMap:=
-  init_mem 0x500 := 0x20;
-  init_mem 0x501 := 0x00;
-  init_mem 0x502 := 0x02;
-  init_mem 0x503 := 0xca;
-  init_mem _ := 0x00.
+Definition init_reg : registerMap :=
+  ∅
+  |> reg_insert _PC 0x500
+  |> reg_insert R0 0x0
+  |> reg_insert R1 0x11
+  |> reg_insert R2 0x101.
 
-Definition termCond : terminationCondition 1 := (λ tid rm, rm _PC =? (0x504 : bv 64)).
+Definition init_mem : memoryMap:=
+  ∅
+  |> mem_insert 0x500 4 0xca020020. (* EOR X0, X1, X2 *)
+
+Definition termCond : terminationCondition 1 :=
+  (λ tid rm, reg_lookup _PC rm =? Some (0x504 : bv 64)).
 
 Definition initState :=
   {|MState.state :=
@@ -53,20 +53,19 @@ Qed.
 End EOR.
 
 Module LDR. (* LDR X0, [X1, X0] at 0x500, loading from 0x1000 *)
-Equations init_reg : registerMap:=
-  init_reg (GReg (R_bitvector_64 _PC)) := 0x500;
-  init_reg (GReg (R_bitvector_64 R0)) := 0x1000;
-  init_reg _ := 0x0.
+Definition init_reg : registerMap :=
+  ∅
+  |> reg_insert _PC 0x500
+  |> reg_insert R0 0x1000
+  |> reg_insert R1 0x0.
 
-Equations init_mem : memoryMap:=
-  init_mem 0x500 := 0x20; (* 0010 0000 *)
-  init_mem 0x501 := 0x68; (* 0110 1000 *)
-  init_mem 0x502 := 0x60; (* 0110 0000 *)
-  init_mem 0x503 := 0xF8; (* 1111 1000 *)
-  init_mem 0x1000 := 0x2a;
-  init_mem _ := 0x00.
+Definition init_mem : memoryMap:=
+  ∅
+  |> mem_insert 0x500 4 0xf8606820 (* LDR X0, [X1, X0] *)
+  |> mem_insert 0x1000 8 0x2a. (* data to be read *)
 
-Definition termCond : terminationCondition 1 := (λ tid rm, rm _PC =? (0x504 : bv 64)).
+Definition termCond : terminationCondition 1 :=
+  (λ tid rm, reg_lookup _PC rm =? Some (0x504 : bv 64)).
 
 Definition initState :=
   {|MState.state :=
@@ -83,25 +82,21 @@ Qed.
 End LDR.
 
 Module STRLDR. (* STR X2, [X1, X0]; LDR X0, [X1, X0] at 0x500, using address 0x1100 *)
-  Equations init_reg : registerMap:=
-    init_reg (GReg (R_bitvector_64 _PC)) := 0x500;
-    init_reg (GReg (R_bitvector_64 R0)) := 0x1000;
-    init_reg (GReg (R_bitvector_64 R1)) := 0x100;
-    init_reg (GReg (R_bitvector_64 R2)) := 0x2a;
-    init_reg _ := 0x0.
+  Definition init_reg : registerMap :=
+    ∅
+    |> reg_insert _PC 0x500
+    |> reg_insert R0 0x1000
+    |> reg_insert R1 0x100
+    |> reg_insert R2 0x2a.
 
-  Equations init_mem : memoryMap:=
-    init_mem 0x500 := 0x22; (* 0010 0010 *)
-    init_mem 0x501 := 0x68; (* 0110 1000 *)
-    init_mem 0x502 := 0x20; (* 0010 0000 *)
-    init_mem 0x503 := 0xF8; (* 1111 1000 *)
-    init_mem 0x504 := 0x20; (* 0010 0000 *)
-    init_mem 0x505 := 0x68; (* 0110 1000 *)
-    init_mem 0x506 := 0x60; (* 0110 0000 *)
-    init_mem 0x507 := 0xF8; (* 1111 1000 *)
-    init_mem _ := 0x00.
+  Definition init_mem : memoryMap:=
+    ∅
+    |> mem_insert 0x500 4 0xf8206822 (* STR X2, [X1, X0] *)
+    |> mem_insert 0x504 4 0xf8606820 (* LDR X0, [X1, X0] *)
+    |> mem_insert 0x1100 8 0x0. (* Memory need to exists to be written to *)
 
-  Definition termCond : terminationCondition 1 := (λ tid rm, rm _PC =? (0x508 : bv 64)).
+  Definition termCond : terminationCondition 1 :=
+    (λ tid rm, reg_lookup _PC rm =? Some (0x508 : bv 64)).
 
   Definition initState :=
     {|MState.state :=
